should be fixed

flightBackend.dfy
@@ -1,5 +1,3 @@
-
-
 datatype preferences = Time | Cost | ffPoint
 
 
@@ -157,7 +155,7 @@ class Graph {
 	}
 
 	method getIndex(citys: seq<City>, searchingFor: City) returns (z : int)
-		requires citys != [];
+		//requires citys != [];
 		requires searchingFor != null;
 		ensures z < |citys|;
 		{
@@ -183,7 +181,6 @@ class Graph {
 	
 predicate correctQuery(q: Query)
     reads q;
-
 {
     q != null && q.start != null && q.end != null
 }
@@ -191,58 +188,21 @@ predicate correctQuery(q: Query)
 predicate correctCities(cities: seq<City>)
     reads cities;
 {
-    cities != [] && null !in cities && forall c: City | c in cities :: null !in c.flights
+    null !in cities && forall c: City | c in cities :: null !in c.flights
 }
 
-//following predicates are used to justify the closedGraph one, which helps with search
-//however..there an issue with reads clause that is not allowing me to access things..
-//should appear as: all c: City :: c == graph.cities[x].flight[x].end ==> c in graph.cities
-//should appear as: all c: City :: c == graph.cities[x].flight[x].start ==> c in graph.cities
-//should appear as: all c: City :: c in graph.cities ==> c == graph.cities[x].flight[x].end
-//should appear as: all c: City :: c in graph.cities ==> c == graph.cities[x].flight[x].end
-function method flightsInGraph (f: Flight, g:Graph) : bool
-	reads f;
-	reads g;
-	{
-		g != null && f != null && f.end in g.cities && f.start in g.cities
-	}
-
-function method citiesFlightInGraph(f: seq<Flight>, g: Graph) : bool
-	reads g;
-	reads f;
-	reads if forall i: nat | i < |f| :: null != f[i] then f[..] else [] 
+predicate flightInGraph(f: Flight, g: Graph)
+    reads f, g;
 {
-<<<<<<< HEAD
     g != null && f != null && f.end in g.cities && f.start in g.cities && 
 		exists t: City | t in g.cities :: t == f.end && exists t: City | t in g.cities :: t == f.start
-=======
-	g != null && null !in f && forall i: nat | i < |f| :: flightsInGraph(f[i] , g)
->>>>>>> cooldudes
 }
 
-function method cityInGraph(c: City, g: Graph) : bool
-	reads g;
-	reads c;
-	requires c != null
-	reads if c != null && forall i: nat | i < |c.flights| :: null !in c.flights then c.flights else [] 
-	reads if c != null then c.flights[..] else []
-{	
-	g != null && c != null && null !in c.flights && 
-	forall i: nat | i < |c.flights| :: citiesFlightInGraph(c.flights, g) && 
-	(exists x: City | x in g.cities :: x == c) &&
-	(exists x: City | x in g.cities :: c == x)
-}
-
-predicate closedGraph(g: Graph) //usually passing City.flights and Graphs.cities
-	reads g;
-{
-	g != null && null !in g.cities && forall i: nat | i < | g.cities | :: cityInGraph(g.cities[i], g)
-}
-	
 method getFlightSolutions(query: Query, g: Graph) returns (flightList: seq<Trip>)
 	requires correctQuery(query);
     requires g != null;
     requires correctCities(g.cities);
+    requires forall c: City | c in g.cities :: forall f: Flight | f in c.flights :: flightInGraph(f, g);
     //ensures that flightList matches the spec!
 {
 
@@ -257,7 +217,7 @@ method searchFlights(query: Query, g: Graph) returns (solutions: seq<Trip>)
     requires correctQuery(query);
     requires g != null;
     requires correctCities(g.cities);
-	//ensures |g.cities| ;
+    requires forall c: City | c in g.cities :: forall f: Flight | f in c.flights :: flightInGraph(f, g);
 {
     var openQueue := new Queue<Trip>.init();
     var closedSet: set<Trip>;
